updated Launchbury entry

thys/Launchbury/HOLCF-Utils.thy
@@ -1,5 +1,87 @@
 theory "HOLCF-Utils"
-  imports HOLCF
+  imports HOLCF Pointwise
 begin
+
+default_sort type
+
+lemmas cont_fun[simp]
+lemmas cont2cont_fun[simp]
+
+lemma cont_compose2:
+  assumes "cont c"
+  assumes "\<And> x. cont (c x)"
+  assumes "cont f"
+  assumes "cont g"
+  shows "cont (\<lambda>x. c (f x) (g x))"
+  by (rule cont_apply[OF assms(4) assms(2) cont2cont_fun[OF cont_compose[OF assms(1) assms(3)]]])
+
+lemma pointwise_adm:
+  fixes P :: "'a::pcpo \<Rightarrow> 'b::pcpo \<Rightarrow> bool"
+  assumes "adm (\<lambda> x. P (fst x) (snd x))"
+  shows "adm (\<lambda> m. pointwise P (fst m) (snd m))"
+proof (rule admI)
+  case (goal1 Y)
+    show ?case
+    apply (rule pointwiseI)
+    apply (rule admD[OF adm_subst[where t = "\<lambda>p . (fst p x, snd p x)", standard, OF _ assms, simplified] `chain Y`])
+    using goal1(2) unfolding pointwise_def by auto
+qed
+
+lemma fun_upd_mono:
+  "\<rho>1 \<sqsubseteq> \<rho>2 \<Longrightarrow> v1 \<sqsubseteq> v2 \<Longrightarrow> \<rho>1(x := v1) \<sqsubseteq> \<rho>2(x := v2)"
+  apply (rule fun_belowI)
+  apply (case_tac "xa = x")
+  apply simp
+  apply (auto elim:fun_belowD)
+  done
+
+lemma fun_upd_cont[simp,cont2cont]:
+  assumes "cont f" and "cont h"
+  shows "cont (\<lambda> x. (f x)(v := h x) :: 'a \<Rightarrow> 'b::pcpo)"
+  by (rule cont2cont_lambda)(auto simp add: assms)
+
+
+subsubsection {* Composition of fun and cfun *}
+
+lemma cont2cont_comp [simp, cont2cont]:
+  assumes "cont f"
+  assumes "\<And> x. cont (f x)"
+  assumes "cont g"
+  shows "cont (\<lambda> x. (f x) \<circ> (g x))"
+  unfolding comp_def
+  by (rule cont2cont_lambda)
+     (intro cont2cont  `cont g` `cont f` cont_compose2[OF assms(1,2)] cont2cont_fun)
+
+definition cfun_comp :: "('a::pcpo \<rightarrow> 'b::pcpo) \<rightarrow> ('c::type \<Rightarrow> 'a) \<rightarrow> ('c::type \<Rightarrow> 'b)"
+  where  "cfun_comp = (\<Lambda> f \<rho>. (\<lambda> x. f\<cdot>x) \<circ> \<rho>)"
+
+lemma [simp]: "cfun_comp\<cdot>f\<cdot>(\<rho>(x := v)) = (cfun_comp\<cdot>f\<cdot>\<rho>)(x := f\<cdot>v)"
+  unfolding cfun_comp_def by auto
+
+lemma cfun_comp_app[simp]: "(cfun_comp\<cdot>f\<cdot>\<rho>) x = f\<cdot>(\<rho> x)"
+  unfolding cfun_comp_def by auto
+
+lemma fix_eq_fix:
+  "f\<cdot>(fix\<cdot>g) \<sqsubseteq> fix\<cdot>g \<Longrightarrow> g\<cdot>(fix\<cdot>f) \<sqsubseteq> fix\<cdot>f \<Longrightarrow> fix\<cdot>f = fix\<cdot>g"
+  by (metis fix_least_below below_antisym)
+
+subsection {* Additional transitivity rules *}
+
+text {*
+These collect side-conditions of the form @{term "cont f"}, so the usual way to discharge them
+is to write @{text[source] "by this (intro cont2cont)+"} at the end.
+*}
+
+lemma below_trans_cong[trans]:
+  "a \<sqsubseteq> f x \<Longrightarrow> x \<sqsubseteq> y \<Longrightarrow> cont f \<Longrightarrow> a \<sqsubseteq> f y "
+by (metis below_trans cont2monofunE)
+
+lemma not_bot_below_trans[trans]:
+  "a \<noteq> \<bottom> \<Longrightarrow> a \<sqsubseteq> b \<Longrightarrow> b \<noteq> \<bottom>"
+  by (metis below_bottom_iff)
+
+lemma not_bot_below_trans_cong[trans]:
+  "f a \<noteq> \<bottom> \<Longrightarrow> a \<sqsubseteq> b \<Longrightarrow> cont f \<Longrightarrow> f b \<noteq> \<bottom>"
+  by (metis below_bottom_iff cont2monofunE)
 
 end
