thys/Launchbury/Terms.thy
@@ -1,19 +1,24 @@
 theory Terms
-  imports Main  "./Nominal/Nominal/Nominal2" 
+  imports "Nominal-Utils" Vars  "AList-Utils-Nominal"
 begin
 
-subsubsection {* Variables (names) and expressions *}
+subsubsection {* Expressions *}
 
 text {*
-The type of variables is abstract and provided by the Nominal package. All we know is that it is countable.
-*}
+This is the main data type of the development; our minimal lambda calculus with recursive let-bindings.
+It is created using the nominal\_datatype command, which creates alpha-equivalence classes.
 
-atom_decl var
+The package does not support nested recursion, so the bindings of the let cannot simply be of type
+@{text "(var, exp) list"}. Instead, the definition of lists have to be inlined here, as the custom type
+@{text "assn"}. Later we create conversion functions between these two types, define a properly typed @{text let} 
+and redo the various lemmas in terms of that, so that afterwards, the type @{text "assn"} is no longer
+referenced.
+*}
 
 nominal_datatype exp =
   Var "var"
 | App "exp" "var"
-| Let as::"assn" body::"exp" binds "bn as" in "body" "as"
+| LetA as::"assn" body::"exp" binds "bn as" in "body" "as"
 | Lam x::"var" body::"exp" binds x in body  ("Lam [_]. _" [100, 100] 100)
 and assn =
   ANil | ACons "var" "exp" "assn" 
@@ -23,15 +28,249 @@ where "bn ANil = []" | "bn (ACons x t as) = (atom x) # (bn as)"
 
 notation (latex output) Terms.Var ("_")
 notation (latex output) Terms.App ("_ _")
-notation (latex output) Terms.Let ("\<^raw:\textrm{\textsf{let}}> _ \<^raw:\textrm{\textsf{in}}> _")
-notation (latex output) Terms.Lam ("\<lambda>_. _")
+notation (latex output) Terms.Lam ("\<lambda>_. _"  [100, 100] 100)
+
+type_synonym heap = "(var \<times> exp) list"
+
+subsubsection {* Rewriting in terms of heaps *}
+
+text {*
+We now work towards using @{type heap} instead of @{type assn}. All this
+could be skipped if Nominal supported nested recursion.
+*}
+
+text {*
+Conversion from @{typ assn} to @{typ heap}.
+*}
+
+nominal_primrec asToHeap :: "assn \<Rightarrow> heap" 
+ where ANilToHeap: "asToHeap ANil = []"
+ | AConsToHeap: "asToHeap (ACons v e as) = (v, e) # asToHeap as"
+unfolding eqvt_def asToHeap_graph_aux_def
+apply rule
+apply simp
+apply rule
+apply(case_tac x rule: exp_assn.exhaust(2))
+apply auto
+done
+termination(eqvt) by lexicographic_order
+
+lemma asToHeap_eqvt: "eqvt asToHeap"
+  unfolding eqvt_def
+  by (auto simp add: permute_fun_def asToHeap.eqvt)
+
+text {* The other direction. *}
+
+fun heapToAssn :: "heap \<Rightarrow> assn"
+  where "heapToAssn [] = ANil" 
+  | "heapToAssn ((v,e)#\<Gamma>) = ACons v e (heapToAssn \<Gamma>)"
+declare heapToAssn.simps[simp del]
+
+lemma heapToAssn_eqvt[simp,eqvt]: "p \<bullet> heapToAssn \<Gamma> =  heapToAssn (p \<bullet> \<Gamma>)"
+  by (induct \<Gamma> rule: heapToAssn.induct)
+     (auto simp add: heapToAssn.simps)
+
+lemma bn_heapToAssn: "bn (heapToAssn \<Gamma>) = map (\<lambda>x. atom (fst x)) \<Gamma>"
+  by (induct rule: heapToAssn.induct)
+     (auto simp add: heapToAssn.simps exp_assn.bn_defs)
+
+lemma set_bn_to_atom_domA:
+  "set (bn as) = atom ` domA (asToHeap as)"
+   by (induct as rule: asToHeap.induct)
+      (auto simp add: exp_assn.bn_defs)
+
+text {*
+They are inverse to each other.
+*}
+
+lemma heapToAssn_asToHeap[simp]:
+  "heapToAssn (asToHeap as) = as"
+  by (induct  rule: exp_assn.inducts(2)[of "\<lambda> _ . True"])
+     (auto simp add: heapToAssn.simps)
+
+lemma asToHeap_heapToAssn[simp]:
+  "asToHeap (heapToAssn as) = as"
+  by (induct rule: heapToAssn.induct)
+     (auto simp add: heapToAssn.simps)
+
+lemma heapToAssn_inject[simp]:
+  "heapToAssn x = heapToAssn y \<longleftrightarrow> x = y"
+  by (metis asToHeap_heapToAssn)
+
+text {*
+They are transparent to varios notions from the Nominal package.
+*}
+
+lemma supp_heapToAssn: "supp (heapToAssn \<Gamma>) = supp \<Gamma>"
+  by (induct rule: heapToAssn.induct)
+     (simp_all add: heapToAssn.simps  exp_assn.supp supp_Nil supp_Cons supp_Pair sup_assoc)
+
+lemma supp_asToHeap: "supp (asToHeap as) = supp as"
+   by (induct as rule: asToHeap.induct)
+      (simp_all add:  exp_assn.supp supp_Nil supp_Cons supp_Pair sup_assoc)
+
+lemma fv_asToHeap: "fv (asToHeap \<Gamma>) = fv \<Gamma>"
+  unfolding fv_def by (auto simp add: supp_asToHeap)
+
+lemma fv_heapToAssn: "fv (heapToAssn \<Gamma>) = fv \<Gamma>"
+  unfolding fv_def by (auto simp add: supp_heapToAssn)
+
+lemma [simp]: "size (heapToAssn \<Gamma>) = list_size (\<lambda> (v,e) . size e) \<Gamma>"
+  by (induct rule: heapToAssn.induct)
+     (simp_all add: heapToAssn.simps)
+
+text {* Now we define the Let constructor in the form that we actually want. *}
+
+hide_const HOL.Let
+definition Let :: "heap \<Rightarrow> exp \<Rightarrow> exp"
+  where "Let \<Gamma> e = LetA (heapToAssn \<Gamma>) e"
+
+notation (latex output) Let ("\<^raw:\textrm{\textsf{let}}> _ \<^raw:\textrm{\textsf{in}}> _")
 
 abbreviation
   LetBe :: "var\<Rightarrow>exp\<Rightarrow>exp\<Rightarrow>exp" ("let _ be _ in _ " [100,100,100] 100)
 where
-  "let x be t1 in t2 \<equiv> Let (ACons x t1 ANil) t2"
+  "let x be t1 in t2 \<equiv> Let [(x,t1)] t2"
 
-type_synonym heap = "(var \<times> exp) list"
+text {*
+We rewrite all (relevant) lemmas about @{term LetA} in terms of @{term Let}.
+*}
+
+lemma size_Let[simp]: "size (Let \<Gamma> e) = list_size (\<lambda>p. size (snd p)) \<Gamma> + size e + Suc 0"
+  unfolding Let_def by (auto simp add: split_beta')
+
+lemma Let_distinct[simp]:
+  "Var v \<noteq> Let \<Gamma> e"
+  "Let \<Gamma> e \<noteq> Var v"
+  "App e v \<noteq> Let \<Gamma> e'"
+  "Lam [v]. e' \<noteq> Let \<Gamma> e"
+  "Let \<Gamma> e \<noteq> Lam [v]. e'"
+  "Let \<Gamma> e' \<noteq> App e v"
+  unfolding Let_def by simp_all
+
+lemma Let_perm_simps[simp,eqvt]:
+  "p \<bullet> Let \<Gamma> e = Let (p \<bullet> \<Gamma>) (p \<bullet> e)"
+  unfolding Let_def by simp
+
+lemma Let_supp:
+  "supp (Let \<Gamma> e) = (supp e \<union> supp \<Gamma>) - atom ` (domA \<Gamma>)"
+  unfolding Let_def by (simp add: exp_assn.supp supp_heapToAssn bn_heapToAssn domA_def image_image)
+
+lemma Let_fresh[simp]:
+  "a \<sharp> Let \<Gamma> e = (a \<sharp> e \<and> a \<sharp> \<Gamma> \<or> a \<in> atom ` domA \<Gamma>)"
+  unfolding fresh_def by (auto simp add: Let_supp)
+
+lemma Abs_eq_cong:
+  assumes "\<And> p. (p \<bullet> x = x') \<longleftrightarrow> (p \<bullet> y = y')"
+  assumes "supp y = supp x"
+  assumes "supp y' = supp x'"
+  shows "([a]lst. x = [a']lst. x') \<longleftrightarrow> ([a]lst. y = [a']lst. y')"
+  by (simp add: Abs_eq_iff alpha_lst assms)
+
+lemma Let_eq_iff[simp]:
+  "(Let \<Gamma> e = Let \<Gamma>' e') = ([map (\<lambda>x. atom (fst x)) \<Gamma> ]lst. (e, \<Gamma>) = [map (\<lambda>x. atom (fst x)) \<Gamma>']lst. (e',\<Gamma>'))"
+  unfolding Let_def 
+  apply (simp add: bn_heapToAssn)
+  apply (rule Abs_eq_cong)
+  apply (simp_all add: supp_Pair supp_heapToAssn)
+  done
+
+lemma exp_strong_exhaust:
+  fixes c :: "'a :: fs"
+  assumes "(\<And>var. y = Var var \<Longrightarrow> P)"
+  assumes "\<And>exp var. y = App exp var \<Longrightarrow> P"
+  assumes "\<And>\<Gamma> exp. atom ` domA \<Gamma> \<sharp>* c \<Longrightarrow> y = Let \<Gamma> exp \<Longrightarrow> P"
+  assumes "\<And>var exp. {atom var} \<sharp>* c \<Longrightarrow> y = Lam [var]. exp \<Longrightarrow> P"
+  shows P
+  apply (rule  exp_assn.strong_exhaust(1)[where y = y and c = c])
+  apply (metis assms(1))
+  apply (metis assms(2))
+  apply (metis assms(3) set_bn_to_atom_domA Let_def heapToAssn_asToHeap)
+  apply (metis assms(4))
+  done
+
+text {*
+And finally the induction rules with @{term Let}.
+*}
+
+lemma exp_heap_induct[case_names Var App Let Lam Nil Cons]:
+  assumes "\<And>var. P1 (Var var)"
+  assumes "\<And>exp var. P1 exp \<Longrightarrow> P1 (App exp var)"
+  assumes "\<And>\<Gamma> exp. P2 \<Gamma> \<Longrightarrow> P1 exp \<Longrightarrow> P1 (Let \<Gamma> exp)"
+  assumes "\<And>var exp. P1 exp \<Longrightarrow> P1 (Lam [var]. exp)"
+  assumes "P2 []"
+  assumes "\<And>var exp \<Gamma>. P1 exp \<Longrightarrow> P2 \<Gamma> \<Longrightarrow> P2 ((var, exp)#\<Gamma>)"
+  shows "P1 e" and "P2 \<Gamma>"
+proof-
+  have "P1 e" and "P2 (asToHeap (heapToAssn \<Gamma>))"
+    apply (induct rule: exp_assn.inducts[of P1 "\<lambda> assn. P2 (asToHeap assn)"])
+    apply (metis assms(1))
+    apply (metis assms(2))
+    apply (metis assms(3) Let_def heapToAssn_asToHeap )
+    apply (metis assms(4))
+    apply (metis assms(5) asToHeap.simps(1))
+    apply (metis assms(6) asToHeap.simps(2))
+    done
+  thus "P1 e" and "P2 \<Gamma>" unfolding asToHeap_heapToAssn.
+qed
+
+lemma exp_heap_strong_induct[case_names Var App Let Lam Nil Cons]:
+  assumes "\<And>var c. P1 c (Var var)"
+  assumes "\<And>exp var c. (\<And>c. P1 c exp) \<Longrightarrow> P1 c (App exp var)"
+  assumes "\<And>\<Gamma> exp c. atom ` domA \<Gamma> \<sharp>* c \<Longrightarrow> (\<And>c. P2 c \<Gamma>) \<Longrightarrow> (\<And>c. P1 c exp) \<Longrightarrow> P1 c (Let \<Gamma> exp)"
+  assumes "\<And>var exp c. {atom var} \<sharp>* c \<Longrightarrow> (\<And>c. P1 c exp) \<Longrightarrow> P1 c (Lam [var]. exp)"
+  assumes "\<And>c. P2 c []"
+  assumes "\<And>var exp \<Gamma> c. (\<And>c. P1 c exp) \<Longrightarrow> (\<And>c. P2 c \<Gamma>) \<Longrightarrow> P2 c ((var,exp)#\<Gamma>)"
+  fixes c :: "'a :: fs"
+  shows "P1 c e" and "P2 c \<Gamma>"
+proof-
+  have "P1 c e" and "P2 c (asToHeap (heapToAssn \<Gamma>))"
+    apply (induct rule: exp_assn.strong_induct[of P1 "\<lambda> c assn. P2 c (asToHeap assn)"])
+    apply (metis assms(1))
+    apply (metis assms(2))
+    apply (metis assms(3) set_bn_to_atom_domA Let_def heapToAssn_asToHeap )
+    apply (metis assms(4))
+    apply (metis assms(5) asToHeap.simps(1))
+    apply (metis assms(6) asToHeap.simps(2))
+    done
+  thus "P1 c e" and "P2 c \<Gamma>" unfolding asToHeap_heapToAssn.
+qed
+
+subsubsection {* Nice induction rules *}
+
+text {*
+These rules can be used instead of the original induction rules, which require a separate
+goal for @{typ assn}.
+*}
+
+lemma exp_induct[case_names Var App Let Lam]:
+  assumes "\<And>var. P (Var var)"
+  assumes "\<And>exp var. P exp \<Longrightarrow> P (App exp var)"
+  assumes "\<And>\<Gamma> exp. (\<And> x. x \<in> domA \<Gamma> \<Longrightarrow>  P (the (map_of \<Gamma> x))) \<Longrightarrow> P exp \<Longrightarrow> P (Let \<Gamma> exp)"
+  assumes "\<And>var exp.  P exp \<Longrightarrow> P (Lam [var]. exp)"
+  shows "P  exp"
+  apply (rule exp_heap_induct[of P "\<lambda> \<Gamma>. (\<forall>x \<in> domA \<Gamma>. P (the (map_of \<Gamma> x)))"])
+  apply (metis assms(1))
+  apply (metis assms(2))
+  apply (metis assms(3))
+  apply (metis assms(4))
+  apply auto
+  done
+
+lemma  exp_strong_induct[case_names Var App Let Lam]:
+  assumes "\<And>var c. P c (Var var)"
+  assumes "\<And>exp var c. (\<And>c. P c exp) \<Longrightarrow> P c (App exp var)"
+  assumes "\<And>\<Gamma> exp c.
+    atom ` domA \<Gamma> \<sharp>* c \<Longrightarrow> (\<And>c x. x \<in> domA \<Gamma> \<Longrightarrow>  P c (the (map_of \<Gamma> x))) \<Longrightarrow> (\<And>c. P c exp) \<Longrightarrow> P c (Let \<Gamma> exp)"
+  assumes "\<And>var exp c. {atom var} \<sharp>* c \<Longrightarrow> (\<And>c. P c exp) \<Longrightarrow> P c (Lam [var]. exp)"
+  shows "P (c::'a::fs) exp"
+  apply (rule exp_heap_strong_induct(1)[of P "\<lambda> c \<Gamma>. (\<forall>x \<in> domA \<Gamma>. P c (the (map_of \<Gamma> x)))"])
+  apply (metis assms(1))
+  apply (metis assms(2))
+  apply (metis assms(3))
+  apply (metis assms(4))
+  apply auto
+  done
 
 subsubsection {* Testing alpha equivalence *}
               
@@ -41,221 +280,52 @@ lemma alpha_test:
 
 lemma alpha_test2:
   shows "let x be (Var x) in (Var x) = let y be (Var y) in (Var y)"
-  by (simp add: exp_assn.bn_defs Abs1_eq_iff fresh_Pair add: fresh_at_base)
+  by (simp add: fresh_Cons fresh_Nil Abs1_eq_iff fresh_Pair add: fresh_at_base)
 
 lemma alpha_test3:
   shows "
-    Let (ACons x (Var y) (ACons y (Var x) ANil)) (Var x)
+    Let [(x, Var y), (y, Var x)] (Var x)
     =
-    Let (ACons y (Var x) (ACons x (Var y) ANil)) (Var y)" (is "Let ?la ?lb = _")
-  apply (simp add: exp_assn.bn_defs Abs1_eq_iff fresh_Pair add:fresh_at_base)
-  apply (simp add: Abs_swap2[of "atom x" "(?lb,?la)" "[atom x, atom y]" "atom y"])
-done
+    Let [(y, Var x), (x, Var y)] (Var y)" (is "Let ?la ?lb = _")
+  by (simp add: bn_heapToAssn Abs1_eq_iff fresh_Pair fresh_at_base
+                Abs_swap2[of "atom x" "(?lb, [(x, Var y), (y, Var x)])" "[atom x, atom y]" "atom y"])
 
-subsubsection {* Substitution *}
+subsubsection {* Free variables *}
 
-fun subst_var :: "var \<Rightarrow> var \<Rightarrow> var \<Rightarrow> var" ("_[_::v=_]" [1000,100,100] 1000)
-where "x[y ::v= z] = (if x = y then z else x)"
+lemma fv_supp_exp: "supp e = atom ` (fv (e::exp) :: var set)" and fv_supp_as: "supp as = atom ` (fv (as::assn) :: var set)"
+  by (induction e and as rule:exp_assn.inducts)
+     (auto simp add: fv_def exp_assn.supp supp_at_base)
 
-lemma subst_var_eqvts[eqvt]:
- fixes \<pi>::perm
- shows "\<pi> \<bullet> (subst_var x y z) = subst_var (\<pi> \<bullet> x) (\<pi> \<bullet> y) (\<pi> \<bullet> z)"
-by auto
+lemma fv_supp_heap: "supp (\<Gamma>::heap) = atom ` (fv \<Gamma> :: var set)"
+  by (metis fv_def fv_supp_as supp_heapToAssn)
 
-(* Helper lemmas provided by Christian Urban *)
+lemma fv_Lam[simp]: "fv (Lam [x]. e) = fv e - {x}"
+  unfolding fv_def by (auto simp add: exp_assn.supp)
+lemma fv_Var[simp]: "fv (Var x) = {x}"
+  unfolding fv_def by (auto simp add: exp_assn.supp supp_at_base)
+lemma fv_App[simp]: "fv (App e x) = insert x (fv e)"
+  unfolding fv_def by (auto simp add: exp_assn.supp supp_at_base)
+lemma fv_Let[simp]: "fv (Let \<Gamma> e) = (fv \<Gamma> \<union> fv e) - domA \<Gamma>"
+  unfolding fv_def by (auto simp add: Let_supp exp_assn.supp supp_at_base set_bn_to_atom_domA)
 
-lemma Projl_permute:
-  assumes a: "\<exists>y. f = Inl y"
-  shows "(p \<bullet> (Sum_Type.Projl f)) = Sum_Type.Projl (p \<bullet> f)"
-using a by auto
+lemma finite_fv_exp[simp]: "finite (fv (e::exp) :: var set)"
+  and finite_fv_heap[simp]: "finite (fv (\<Gamma> :: heap) :: var set)"
+  by (induction e rule:exp_heap_induct) auto
 
-lemma Projr_permute:
-  assumes a: "\<exists>y. f = Inr y"
-  shows "(p \<bullet> (Sum_Type.Projr f)) = Sum_Type.Projr (p \<bullet> f)"
-using a by auto
+lemma fv_not_fresh: "atom x \<sharp> e \<longleftrightarrow> x \<notin> fv e"
+  unfolding fv_def fresh_def by blast
 
-nominal_primrec  (default "sum_case (\<lambda>x. Inl undefined) (\<lambda>x. Inr undefined)",
-                  invariant "\<lambda> a r . (\<forall> as y z . ((a = Inr (as, y, z) \<and> set (bn as) \<sharp>* (y, z)) \<longrightarrow> bn (Sum_Type.Projr r) = bn as))")
-  subst :: "exp \<Rightarrow> var \<Rightarrow> var \<Rightarrow> exp" ("_[_::=_]" [1000,100,100] 1000)
-and
-  subst_assn :: "assn \<Rightarrow> var \<Rightarrow> var \<Rightarrow> assn" ("_[_::a=_]" [1000,100,100] 1000)
-where
-  "(Var x)[y ::= z] = (Var (x[y ::v= z]))"
- |"(App e v)[y ::= z] = (App (e[y ::= z]) (v[y ::v= z]))"
- |"(set (bn as)) \<sharp>* (y,z) \<Longrightarrow> (Let as body)[y ::= z] = Let (subst_assn as y z) (body[y ::= z])" 
- |"(atom x \<sharp> (y,z)) \<Longrightarrow> (Lam [x].e)[y ::= z] = Lam [x].(e[y::=z])"
- |"subst_assn ANil y z = ANil"
- |"subst_assn (ACons v e as) y z = ACons v (e[y ::= z]) (subst_assn as y z)"
+lemma fv_delete_heap:
+  assumes "map_of \<Gamma> x = Some e"
+  shows "fv (delete x \<Gamma>, e) \<union> {x} \<subseteq> (fv (\<Gamma>, Var x) :: var set)"
 proof-
-
-have eqvt_at_subst: "\<And> e y z . eqvt_at subst_subst_assn_sumC (Inl (e, y, z)) \<Longrightarrow> eqvt_at (\<lambda>(a, b, c). subst a b c) (e, y, z)"
-  apply(simp add: eqvt_at_def subst_def)
-  apply(rule)
-  apply(subst Projl_permute)
-  apply(thin_tac "?X")+
-  apply (simp add: subst_subst_assn_sumC_def)
-  apply (simp add: THE_default_def)
-  apply (case_tac "Ex1 (subst_subst_assn_graph (Inl (e, y, z)))")
-  apply(simp)
-  apply(auto)[1]
-  apply (erule_tac x="x" in allE)
-  apply simp
-  apply(cases rule: subst_subst_assn_graph.cases)
-  apply(assumption)
-  apply(rule_tac x="Sum_Type.Projl x" in exI)
-  apply(clarify)
-  apply (rule the1_equality)
-  apply blast 
-  apply(simp (no_asm) only: Projl.simps)
-  apply(rule_tac x="Sum_Type.Projl x" in exI)
-  apply(clarify)
-  apply (rule the1_equality)
-  apply blast 
-  apply(simp (no_asm) only: Projl.simps)
-  apply(rule_tac x="Sum_Type.Projl x" in exI)
-  apply(clarify)
-  apply (rule the1_equality)
-  apply blast 
-  apply(simp (no_asm) only: Projl.simps)
-  apply(rule_tac x="Sum_Type.Projl x" in exI)
-  apply(clarify)
-  apply (rule the1_equality)
-  apply blast 
-  apply(simp (no_asm) only: Projl.simps)
-  apply (metis Inr_not_Inl)
-  apply (metis Inr_not_Inl)
-  apply(simp)
-  apply(perm_simp)
-  apply(simp)
-done
-
-have eqvt_at_subst_assn: "\<And> as y z . eqvt_at subst_subst_assn_sumC (Inr (as, y, z)) \<Longrightarrow> eqvt_at (\<lambda>(a, b, c). subst_assn a b c) (as, y, z)"
-  apply(simp add: eqvt_at_def subst_assn_def)
-  apply(rule)
-  apply(subst Projr_permute)
-  apply(thin_tac "?X")+
-  apply (simp add: subst_subst_assn_sumC_def)
-  apply (simp add: THE_default_def)
-  apply (case_tac "Ex1 (subst_subst_assn_graph (Inr (as, y, z)))")
-  apply(simp)
-  apply(auto)[1]
-  apply (erule_tac x="x" in allE)
-  apply simp
-  apply(cases rule: subst_subst_assn_graph.cases)
-  apply(assumption)
-  apply (metis (mono_tags) Inr_not_Inl)+
-  apply(rule_tac x="Sum_Type.Projr x" in exI)
-  apply(clarify)
-  apply (rule the1_equality)
-  apply auto[1]
-  apply(simp (no_asm) only: Projr.simps)
-  
-  apply(rule_tac x="Sum_Type.Projr x" in exI)
-  apply(clarify)
-  apply (rule the1_equality)
-  apply auto[1]
-  apply(simp (no_asm) only: Projr.simps)
-  
-  apply(simp)
-  apply(perm_simp)
-  apply(simp)
-done
-
-{
-(* Equivariance of the graph *)
-case goal1 thus ?case
-  unfolding eqvt_def subst_subst_assn_graph_aux_def
-  by simp
-
-(* The invariant *)
-next case goal2 thus ?case
-  by (induct rule: subst_subst_assn_graph.induct)(auto simp add: exp_assn.bn_defs fresh_star_insert)
-
-(* Exhaustiveness *)
-next case (goal3 P x) show ?case
-  proof(cases x)
-  case (Inl a) thus P
-    proof(cases a)
-    case (fields a1 a2 a3)
-    thus P using Inl goal3
-      apply (rule_tac y ="a1" and c ="(a2, a3)" in exp_assn.strong_exhaust(1))
-      apply (auto simp add: fresh_star_def)
-      apply metis
-    done
-  qed
-  next
-  case (Inr a) thus P
-    proof (cases a)
-    case (fields a1 a2 a3)
-    thus P using Inr goal3
-      apply (rule_tac ya ="a1" in exp_assn.strong_exhaust(2))
-      apply (auto)
-      apply blast+
-    done
-  qed
+  have "fv (delete x \<Gamma>) \<subseteq> fv \<Gamma>" by (metis fv_delete_subset)
+  moreover
+  have "(x,e) \<in> set \<Gamma>" by (metis assms map_of_is_SomeD)
+  hence "fv e \<subseteq> fv \<Gamma>" by (metis assms domA_from_set map_of_fv_subset the.simps)
+  moreover
+  have "x \<in> fv (Var x)" by simp
+  ultimately show ?thesis by auto
 qed
-
-next case (goal15 e y2 z2 as e2 y z as2) thus ?case
-  apply -
-  apply (drule eqvt_at_subst)+
-  apply (drule eqvt_at_subst_assn)+
-  apply (simp only: meta_eq_to_obj_eq[OF subst_def, symmetric, unfolded fun_eq_iff]
-    meta_eq_to_obj_eq[OF subst_assn_def, symmetric, unfolded fun_eq_iff])
-  (* No _sum any more at this point! *)
-  apply (auto simp add: Abs_fresh_iff)
-  apply (drule_tac
-    c = "(y, z)" and
-    as = "(bn e)" and
-    bs = "(bn e2)" and
-    f = "\<lambda> a b c . [a]lst. (subst (fst b) y z, subst_assn (snd b) y z )" in Abs_lst_fcb2)
-  apply (simp add: perm_supp_eq fresh_Pair fresh_star_def Abs_fresh_iff)
-  apply (simp)
-  apply (simp)
-  apply (simp add: eqvt_at_def, simp add: fresh_star_Pair perm_supp_eq)
-  apply (simp add: eqvt_at_def, simp add: fresh_star_Pair perm_supp_eq)
-  apply (simp add: eqvt_at_def)
-  done
-
-next case (goal19 x2 y2 z2 e2 x y z e) thus ?case
-  apply -
-  apply (drule eqvt_at_subst)+
-  apply (simp only: Abs_fresh_iff meta_eq_to_obj_eq[OF subst_def, symmetric, unfolded fun_eq_iff])
-  (* No _sum any more at this point! *)
-  apply (simp add: eqvt_at_def)
-  apply rule
-  apply (erule_tac x = "(x2 \<leftrightarrow> c)" in allE)
-  apply (erule_tac x = "(x \<leftrightarrow> c)" in allE)
-  apply auto
-  done
-}
-qed(auto)
-
-termination (eqvt) by lexicographic_order
-
-lemma shows
-  True and bn_subst[simp]: "set (bn as) \<sharp>* (y, z) \<Longrightarrow> bn (subst_assn as y z) = bn as"
-by(induct rule:subst_subst_assn.induct)
-  (auto simp add: exp_assn.bn_defs fresh_star_insert)
-
-
-lemma subst_is_fresh[simp]:
-assumes "atom y \<sharp> z"
-shows
-  "atom y \<sharp> e[y ::= z]"
-and
- "set (bn as) \<sharp>* (y, z) \<Longrightarrow> atom y \<sharp> (subst_assn as y z)"
-using assms
-by(induct e y z and as y z rule:subst_subst_assn.induct)
-  (auto simp add:fresh_at_base fresh_star_Pair exp_assn.bn_defs fresh_star_insert)
-
-lemma
- subst_pres_fresh: "(atom x \<sharp> e \<and> atom x \<sharp> z) --> atom x \<sharp> e[y ::= z]"
-and
- "(atom x \<sharp> as \<and> atom x \<sharp> z \<and> atom x \<notin> set (bn as)) --> (atom x \<sharp> (subst_assn as y z))"
-by(induct e y z and as y z rule:subst_subst_assn.induct)
-  (auto simp add:fresh_at_base fresh_star_Pair exp_assn.bn_defs fresh_star_insert)
-
-lemma let_binders_fresh[simp]: "set (bn as) \<sharp>* Terms.Let as body"
-  by (metis Diff_iff exp_assn.supp(3) finite_supp fresh_finite_atom_set fresh_star_def fresh_star_set fresh_star_supp_conv supp_of_atom_list)
 
 end
