thys/Launchbury/AList-Utils.thy
@@ -1,0 +1,80 @@
+theory "AList-Utils"
+imports Main "Library/AList"
+begin
+
+text {* We want to have @{text delete} and @{text update} back in the namespace. *}
+
+abbreviation delete where "delete \<equiv> AList.delete"
+abbreviation update where "update \<equiv> AList.update"
+
+subsubsection {* The domain of an associative list *}
+
+definition domA
+  where "domA h = fst ` set h"
+
+lemma domA_append[simp]:"domA (a @ b) = domA a \<union> domA b"
+  and [simp]:"domA ((v,e) # h) = insert v (domA h)"
+  and [simp]:"domA (p # h) = insert (fst p) (domA h)"
+  and [simp]:"domA [] = {}"
+  by (auto simp add: domA_def)
+
+lemma domA_from_set:
+  "(x, e) \<in> set h \<Longrightarrow> x \<in> domA h"
+by (induct h, auto)
+
+lemma finite_domA[simp]:
+  "finite (domA \<Gamma>)"
+  by (auto simp add: domA_def)
+
+lemma domA_delete[simp]:
+  "domA (delete x \<Gamma>) = domA \<Gamma> - {x}"
+  by (induct \<Gamma>) auto
+
+lemma delete_not_domA[simp]:
+  "x \<notin> domA \<Gamma> \<Longrightarrow>  delete x \<Gamma> = \<Gamma>"
+  by (induct \<Gamma>) auto
+
+lemma dom_map_of_conv_domA:
+  "dom (map_of \<Gamma>) = domA \<Gamma>"
+  by (induct \<Gamma>) (auto simp add: dom_if)
+
+lemma domA_map_of_Some_the:
+  "x \<in> domA \<Gamma> \<Longrightarrow> map_of \<Gamma> x = Some (the (map_of \<Gamma> x))"
+  by (induct \<Gamma>) (auto simp add: dom_if)
+
+subsubsection {* Other lemmas about associative lists *}
+
+lemma delete_set_none: "(map_of l)(x := None) = map_of (delete x l)"
+proof (induct l)
+  case Nil thus ?case by simp
+  case (Cons l ls)
+  from this[symmetric]
+  show ?case
+  by (cases "fst l = x") auto
+qed
+     
+lemma list_size_delete[simp]: "list_size size (delete x l) < Suc (list_size size l)"
+  by (induct l) auto
+
+lemma delete_append[simp]: "delete x (l1 @ l2) = delete x l1 @ delete x l2"
+  unfolding AList.delete_eq by simp
+
+lemma map_of_delete_insert:
+  assumes "map_of \<Gamma> x = Some e"
+  shows "map_of ((x,e) # delete x \<Gamma>) = map_of \<Gamma>"
+  using assms by (induct \<Gamma>) (auto split:prod.split)
+
+lemma map_add_domA[simp]: 
+  "x \<in> domA \<Gamma> \<Longrightarrow> (map_of \<Delta> ++ map_of \<Gamma>) x = map_of \<Gamma> x"
+  "x \<notin> domA \<Gamma> \<Longrightarrow> (map_of \<Delta> ++ map_of \<Gamma>) x = map_of \<Delta> x"
+    apply (metis dom_map_of_conv_domA map_add_dom_app_simps(1))
+    apply (metis dom_map_of_conv_domA map_add_dom_app_simps(3))
+    done
+
+lemma map_of_empty[simp]:
+  "Map.empty = map_of \<Delta> \<longleftrightarrow> \<Delta> = []"
+  apply (cases \<Delta>)
+  apply auto
+  by (metis fun_upd_same option.distinct(1))
+
+end
