thys/Launchbury/CorrectnessOriginal.thy
@@ -1,0 +1,180 @@
+theory CorrectnessOriginal
+imports "Denotational" "Launchbury"
+begin
+
+text {*
+This is the main correctness theorem, Theorem 2 from \cite{launchbury}.
+*}
+
+(* Another possible invariant seems to be: "edom \<rho> - domA \<Gamma> \<subseteq> set L" *)
+
+theorem correctness:
+  assumes "\<Gamma> : e \<Down>\<^bsub>L\<^esub> \<Delta> : z"
+  and     "fv (\<Gamma>, e) - domA \<Gamma> \<subseteq> set L"
+  shows   "\<lbrakk>e\<rbrakk>\<^bsub>\<lbrace>\<Gamma>\<rbrace>\<rho>\<^esub> = \<lbrakk>z\<rbrakk>\<^bsub>\<lbrace>\<Delta>\<rbrace>\<rho>\<^esub>" and "(\<lbrace>\<Gamma>\<rbrace>\<rho>) f|` domA \<Gamma> = (\<lbrace>\<Delta>\<rbrace>\<rho>) f|` domA \<Gamma>"
+  using assms
+proof(nominal_induct arbitrary: \<rho> rule:reds.strong_induct)
+case Lambda
+  case 1 show ?case..
+  case 2 show ?case..
+next
+case (Application y \<Gamma> e x L \<Delta> \<Theta> z e')
+  hence "y \<noteq> x" by (simp_all add: fresh_at_base)
+
+  have Gamma_subset: "domA \<Gamma> \<subseteq> domA \<Delta>"
+    by (rule reds_doesnt_forget[OF Application.hyps(8)])
+
+  case 1
+  hence prem1: "fv (\<Gamma>, e) - domA \<Gamma> \<subseteq> set (x#L)" by auto
+
+  from 1 Gamma_subset have *: "x \<in> set L \<or> x \<in> domA \<Delta>" by auto
+
+  have "fv (\<Delta>, e'[y::=x]) - domA \<Delta> \<subseteq> (fv (\<Delta>, Lam [y]. e') - domA \<Delta>) \<union> {x}"
+    by (auto dest!: set_mp[OF fv_subst_subset])
+  also have "\<dots> \<subseteq> (fv (\<Gamma>, e) - domA \<Gamma>) \<union> {x}"
+    using new_free_vars_on_heap[OF Application.hyps(8)] by auto
+  also have "\<dots> \<subseteq> set L \<union> {x}" using prem1 by auto
+  finally have "fv (\<Delta>, e'[y::=x]) - domA \<Delta> \<subseteq> set L \<union> {x}". 
+  with *
+  have prem2: "fv (\<Delta>, e'[y::=x]) - domA \<Delta> \<subseteq> set L" by auto
+  
+  have *: "(\<lbrace>\<Gamma>\<rbrace>\<rho>) x = (\<lbrace>\<Delta>\<rbrace>\<rho>) x"
+  proof(cases "x \<in> domA \<Gamma>")
+    case True
+    from Application.hyps(10)[OF prem1, where \<rho> = \<rho>]
+    have "((\<lbrace>\<Gamma>\<rbrace>\<rho>) f|` domA \<Gamma>) x  = ((\<lbrace>\<Delta>\<rbrace>\<rho>) f|` domA \<Gamma>) x" by simp
+    with True show ?thesis by simp
+  next
+    case False 
+    from False reds_avoids_live[OF Application.hyps(8)] 
+    show ?thesis by (simp add: lookup_HSem_other)
+  qed
+
+  have "\<lbrakk> App e x \<rbrakk>\<^bsub>\<lbrace>\<Gamma>\<rbrace>\<rho>\<^esub> = (\<lbrakk> e \<rbrakk>\<^bsub>\<lbrace>\<Gamma>\<rbrace>\<rho>\<^esub>) \<down>Fn (\<lbrace>\<Gamma>\<rbrace>\<rho>) x"
+    by simp
+  also have "\<dots> = (\<lbrakk> Lam [y]. e' \<rbrakk>\<^bsub>\<lbrace>\<Delta>\<rbrace>\<rho>\<^esub>) \<down>Fn (\<lbrace>\<Gamma>\<rbrace>\<rho>) x"
+    using Application.hyps(9)[OF prem1] by simp
+  also have "\<dots> = (\<lbrakk> Lam [y]. e' \<rbrakk>\<^bsub>\<lbrace>\<Delta>\<rbrace>\<rho>\<^esub>) \<down>Fn (\<lbrace>\<Delta>\<rbrace>\<rho>) x"
+    unfolding *..
+  also have "\<dots> = (Fn \<cdot> (\<Lambda> v. \<lbrakk> e' \<rbrakk>\<^bsub>(\<lbrace>\<Delta>\<rbrace>\<rho>)(y := v)\<^esub>)) \<down>Fn (\<lbrace>\<Delta>\<rbrace>\<rho>) x"
+    by simp
+  also have "\<dots> = \<lbrakk> e' \<rbrakk>\<^bsub>(\<lbrace>\<Delta>\<rbrace>\<rho>)(y := (\<lbrace>\<Delta>\<rbrace>\<rho>) x)\<^esub>"
+    by simp
+  also have "\<dots> = \<lbrakk> e'[y ::= x] \<rbrakk>\<^bsub>\<lbrace>\<Delta>\<rbrace>\<rho>\<^esub>"
+    by (rule arg_cong[OF ESem_subst[OF `y \<noteq> x`]])
+  also have "\<dots> = \<lbrakk> z \<rbrakk>\<^bsub>\<lbrace>\<Theta>\<rbrace>\<rho>\<^esub>"
+    by (rule Application.hyps(12)[OF prem2])
+  finally
+  show ?case.
+  
+  show "(\<lbrace>\<Gamma>\<rbrace>\<rho>) f|` domA \<Gamma> = (\<lbrace>\<Theta>\<rbrace>\<rho>) f|` domA \<Gamma>"
+    using Application.hyps(10)[OF prem1]
+          env_restr_eq_subset[OF Gamma_subset Application.hyps(13)[OF prem2]]
+    by (rule trans)
+next
+case (Variable \<Gamma> x e L \<Delta> z)
+  hence [simp]:"x \<in> domA \<Gamma>" by (metis domA_from_set map_of_is_SomeD)
+
+  let ?\<Gamma> = "delete x \<Gamma>"
+
+  case 2
+  have "x \<notin> domA \<Delta>"
+    by (rule reds_avoids_live[OF Variable.hyps(2)], simp_all)
+
+  have subset: "domA ?\<Gamma> \<subseteq> domA \<Delta>"
+    by (rule reds_doesnt_forget[OF Variable.hyps(2)])
+
+  have "fv (?\<Gamma>, e) \<union> {x} \<subseteq> fv (\<Gamma>, Var x)"
+    by (rule fv_delete_heap[OF `map_of \<Gamma> x = Some e`])
+  hence prem: "fv (?\<Gamma>, e) - domA ?\<Gamma> \<subseteq> set (x # L)" using 2 by auto
+
+  have fv_subset: "fv (?\<Gamma>, e) - domA ?\<Gamma> \<subseteq> - (domA \<Delta> - domA \<Gamma>)"
+    apply (rule subset_trans[OF prem])
+    apply (rule subset_trans[OF reds_avoids_live'[OF Variable.hyps(2)]])
+    by auto
+
+  let "?new" = "domA \<Delta> - domA \<Gamma>"
+  have "domA \<Gamma> \<subseteq> (-?new)" by auto
+
+  have "\<lbrace>\<Gamma>\<rbrace>\<rho> = \<lbrace>(x,e) # ?\<Gamma>\<rbrace>\<rho>"
+    by (rule HSem_reorder[OF map_of_delete_insert[symmetric, OF Variable(1)]])
+  also have "\<dots> = (\<mu> \<rho>'. (\<rho> ++\<^bsub>(domA ?\<Gamma>)\<^esub> (\<lbrace>?\<Gamma>\<rbrace>\<rho>'))( x := \<lbrakk> e \<rbrakk>\<^bsub>\<rho>'\<^esub>))"
+    by (rule iterative_HSem, simp)
+  also have "\<dots> = (\<mu> \<rho>'. (\<rho> ++\<^bsub>(domA ?\<Gamma>)\<^esub> (\<lbrace>?\<Gamma>\<rbrace>\<rho>'))( x := \<lbrakk> e \<rbrakk>\<^bsub>\<lbrace>?\<Gamma>\<rbrace>\<rho>'\<^esub>))"
+    by (rule iterative_HSem', simp)
+  finally
+  have "(\<lbrace>\<Gamma>\<rbrace>\<rho>)f|` (- ?new) = (...) f|` (- ?new)" by simp
+  also have "\<dots> = (\<mu> \<rho>'. (\<rho> ++\<^bsub>domA \<Delta>\<^esub> (\<lbrace>\<Delta>\<rbrace>\<rho>'))( x := \<lbrakk> z \<rbrakk>\<^bsub>\<lbrace>\<Delta>\<rbrace>\<rho>'\<^esub>)) f|` (- ?new)"
+  proof (induction rule: parallel_fix_ind[where P ="\<lambda> x y. x f|` (- ?new) = y f|` (- ?new)"])
+    case 1 show ?case by simp
+  next
+    case 2 show ?case ..
+  next
+    case (3 \<sigma> \<sigma>')
+    hence "\<lbrakk> e \<rbrakk>\<^bsub>\<lbrace>?\<Gamma>\<rbrace>\<sigma>\<^esub> = \<lbrakk> e \<rbrakk>\<^bsub>\<lbrace>?\<Gamma>\<rbrace>\<sigma>'\<^esub>"
+      and "(\<lbrace>?\<Gamma>\<rbrace>\<sigma>) f|` domA ?\<Gamma> = (\<lbrace>?\<Gamma>\<rbrace>\<sigma>') f|` domA ?\<Gamma>"
+      using fv_subset by (auto intro: ESem_fresh_cong HSem_fresh_cong  env_restr_eq_subset[OF _ 3])
+    from trans[OF this(1) Variable(3)[OF prem]] trans[OF this(2) Variable(4)[OF prem]]
+    have  "\<lbrakk> e \<rbrakk>\<^bsub>\<lbrace>?\<Gamma>\<rbrace>\<sigma>\<^esub> = \<lbrakk> z \<rbrakk>\<^bsub>\<lbrace>\<Delta>\<rbrace>\<sigma>'\<^esub>"
+       and "(\<lbrace>?\<Gamma>\<rbrace>\<sigma>) f|` domA ?\<Gamma> = (\<lbrace>\<Delta>\<rbrace>\<sigma>') f|` domA ?\<Gamma>".
+    thus ?case
+      using subset
+      by (auto intro!: ext simp add: lookup_override_on_eq  lookup_env_restr_eq dest: env_restr_eqD )
+  qed
+  also have "\<dots> = (\<mu> \<rho>'. (\<rho> ++\<^bsub>domA \<Delta>\<^esub> (\<lbrace>\<Delta>\<rbrace>\<rho>'))( x := \<lbrakk> z \<rbrakk>\<^bsub>\<rho>'\<^esub>)) f|` (-?new)"
+    by (rule arg_cong[OF iterative_HSem'[symmetric], OF `x \<notin> domA \<Delta>`])
+  also have "\<dots> = (\<lbrace>(x,z) # \<Delta>\<rbrace>\<rho>)  f|` (-?new)"
+    by (rule arg_cong[OF iterative_HSem[symmetric], OF `x \<notin> domA \<Delta>`])
+  finally
+  show le: ?case by (rule env_restr_eq_subset[OF `domA \<Gamma> \<subseteq> (-?new)`])
+
+  have "\<lbrakk> Var x \<rbrakk>\<^bsub>\<lbrace>\<Gamma>\<rbrace>\<rho>\<^esub> = \<lbrakk> Var x \<rbrakk>\<^bsub>\<lbrace>(x, z) # \<Delta>\<rbrace>\<rho>\<^esub>"
+    using env_restr_eqD[OF le, where x = x]
+    by simp
+  also have "\<dots> = \<lbrakk> z \<rbrakk>\<^bsub>\<lbrace>(x, z) # \<Delta>\<rbrace>\<rho>\<^esub>"
+    by (auto simp add: lookup_HSem_heap)
+  finally
+  show "\<lbrakk> Var x \<rbrakk>\<^bsub>\<lbrace>\<Gamma>\<rbrace>\<rho>\<^esub> = \<lbrakk> z \<rbrakk>\<^bsub>\<lbrace>(x, z) # \<Delta>\<rbrace>\<rho>\<^esub>".
+next
+case (Let as \<Gamma> L body \<Delta> z)
+  case 1
+  { fix a
+    assume a: "a \<in> domA  as"
+    have "atom a \<sharp> \<Gamma>" 
+      by (rule Let(1)[unfolded fresh_star_def, rule_format, OF imageI[OF a]])
+    hence "a \<notin> domA \<Gamma>"
+      by (metis domA_not_fresh)
+  }
+  note * = this
+
+  
+  have "fv (as @ \<Gamma>, body) - domA (as @ \<Gamma>) \<subseteq>  fv (\<Gamma>, Let as body) - domA \<Gamma>"
+    by auto
+  with 1 have prem: "fv (as @ \<Gamma>, body) - domA (as @ \<Gamma>) \<subseteq> set L" by auto
+  
+  have f1: "atom ` domA as \<sharp>* \<Gamma>"
+    using Let(1) by (simp add: set_bn_to_atom_domA)
+
+  have "\<lbrakk> Let as body \<rbrakk>\<^bsub>\<lbrace>\<Gamma>\<rbrace>\<rho>\<^esub> = \<lbrakk> body \<rbrakk>\<^bsub>\<lbrace>as\<rbrace>\<lbrace>\<Gamma>\<rbrace>\<rho>\<^esub>"
+    by (simp)
+  also have "\<dots> = \<lbrakk> body \<rbrakk>\<^bsub>\<lbrace>as @ \<Gamma>\<rbrace>\<rho>\<^esub>"
+    by (rule arg_cong[OF HSem_merge[OF f1]])
+  also have "\<dots> = \<lbrakk> z \<rbrakk>\<^bsub>\<lbrace>\<Delta>\<rbrace>\<rho>\<^esub>"
+    by (rule Let.hyps(4)[OF prem])
+  finally
+  show ?case.
+
+  have "(\<lbrace>\<Gamma>\<rbrace>\<rho>) f|` (domA \<Gamma>) = (\<lbrace>as\<rbrace>(\<lbrace>\<Gamma>\<rbrace>\<rho>)) f|` (domA \<Gamma>)"
+    apply (rule ext)
+    apply (case_tac "x \<in> domA as")
+    apply (auto simp add: lookup_HSem_other lookup_env_restr_eq *)
+    done
+  also have "\<dots> = (\<lbrace>as @ \<Gamma>\<rbrace>\<rho>) f|` (domA \<Gamma>)"
+    by (rule arg_cong[OF HSem_merge[OF f1]])
+  also have "\<dots> = (\<lbrace>\<Delta>\<rbrace>\<rho>) f|` (domA \<Gamma>)"
+    by (rule env_restr_eq_subset[OF _ Let.hyps(5)[OF prem]]) simp
+  finally
+  show "(\<lbrace>\<Gamma>\<rbrace>\<rho>) f|` domA \<Gamma> = (\<lbrace>\<Delta>\<rbrace>\<rho>) f|` domA \<Gamma>".
+qed
+
+end
