thys/Launchbury/Denotational-Related.thy
@@ -1,0 +1,68 @@
+theory "Denotational-Related"
+imports "Denotational" "ResourcedDenotational" ValueSimilarity
+begin
+
+text {*
+Given the similarity relation it is straight-forward to prove that the standard
+and the resourced denotational semantics produce similar results. (Theorem 10 in
+|cite{functionspaces}).
+*}
+
+theorem denotational_semantics_similar: 
+  assumes "\<rho> \<triangleleft>\<triangleright>\<^sup>* \<sigma>"
+  shows "\<lbrakk>e\<rbrakk>\<^bsub>\<rho>\<^esub> \<triangleleft>\<triangleright> (\<N>\<lbrakk>e\<rbrakk>\<^bsub>\<sigma>\<^esub>)\<cdot>C\<^sup>\<infinity>"
+using assms
+proof(induct e arbitrary: \<rho> \<sigma> rule:exp_induct)
+  case (Var v)
+  hence "\<rho> v \<triangleleft>\<triangleright> (\<sigma> v)\<cdot>C\<^sup>\<infinity>" by cases auto
+  thus ?case by simp
+next
+  case (Lam v e)
+  { fix x y
+    assume "x \<triangleleft>\<triangleright> y\<cdot>C\<^sup>\<infinity>"
+    with `\<rho> \<triangleleft>\<triangleright>\<^sup>* \<sigma>`
+    have "\<rho>(v := x) \<triangleleft>\<triangleright>\<^sup>* \<sigma>(v := y)"
+      by (auto 1 4)
+    hence "\<lbrakk>e\<rbrakk>\<^bsub>\<rho>(v := x)\<^esub> \<triangleleft>\<triangleright> (\<N>\<lbrakk>e\<rbrakk>\<^bsub>\<sigma>(v := y)\<^esub>)\<cdot>C\<^sup>\<infinity>"
+      by (rule Lam.hyps)
+  }
+  thus ?case by auto
+next
+  case (App e v \<rho> \<sigma>)
+  hence App': "\<lbrakk>e\<rbrakk>\<^bsub>\<rho>\<^esub> \<triangleleft>\<triangleright> (\<N>\<lbrakk>e\<rbrakk>\<^bsub>\<sigma>\<^esub>)\<cdot>C\<^sup>\<infinity>" by auto
+  thus ?case
+  proof (cases rule: slimilar_bot_cases)
+    case bot thus ?thesis by auto
+  next
+    case (Fn f g)
+    from `\<rho> \<triangleleft>\<triangleright>\<^sup>* \<sigma>`
+    have "\<rho> v \<triangleleft>\<triangleright> (\<sigma> v)\<cdot>C\<^sup>\<infinity>"  by auto
+    thus ?thesis using Fn App' by auto
+  qed
+next
+  case (Let as e \<rho> \<sigma>)
+  have "\<lbrace>as\<rbrace>\<rho> \<triangleleft>\<triangleright>\<^sup>* \<N>\<lbrace>as\<rbrace>\<sigma>"
+  proof (rule parallel_HSem_ind_different_ESem[OF pointwise_adm[OF similar_admI] fun_similar_fmap_bottom])
+    fix \<rho>' :: "var \<Rightarrow> Value" and \<sigma>' :: "var \<Rightarrow> CValue"
+    assume "\<rho>' \<triangleleft>\<triangleright>\<^sup>* \<sigma>'"
+    show "\<rho> ++\<^bsub>domA as\<^esub> \<^bold>\<lbrakk> as \<^bold>\<rbrakk>\<^bsub>\<rho>'\<^esub> \<triangleleft>\<triangleright>\<^sup>* \<sigma> ++\<^bsub>domA as\<^esub> evalHeap as (\<lambda>e. \<N>\<lbrakk> e \<rbrakk>\<^bsub>\<sigma>'\<^esub>)"
+    proof(rule pointwiseI)
+      case (goal1 x)
+      show ?case using `\<rho> \<triangleleft>\<triangleright>\<^sup>* \<sigma>`
+        by (auto simp add: lookup_override_on_eq lookupEvalHeap elim: Let(1)[OF _  `\<rho>' \<triangleleft>\<triangleright>\<^sup>* \<sigma>'`] )
+    qed
+  qed auto
+  hence "\<lbrakk>e\<rbrakk>\<^bsub>\<lbrace>as\<rbrace>\<rho>\<^esub> \<triangleleft>\<triangleright> (\<N>\<lbrakk>e\<rbrakk>\<^bsub>\<N>\<lbrace>as\<rbrace>\<sigma>\<^esub>)\<cdot>C\<^sup>\<infinity>" by (rule Let(2))
+  thus ?case by simp
+qed
+
+corollary evalHeap_similar:
+  "\<And>y z. y \<triangleleft>\<triangleright>\<^sup>* z \<Longrightarrow> \<^bold>\<lbrakk> \<Gamma> \<^bold>\<rbrakk>\<^bsub>y\<^esub> \<triangleleft>\<triangleright>\<^sup>* \<^bold>\<N>\<lbrakk> \<Gamma> \<^bold>\<rbrakk>\<^bsub>z\<^esub>"
+  by (rule pointwiseI)
+     (case_tac "x \<in> domA \<Gamma>", auto simp add: lookupEvalHeap denotational_semantics_similar)
+
+theorem heaps_similar: "\<lbrace>\<Gamma>\<rbrace> \<triangleleft>\<triangleright>\<^sup>* \<N>\<lbrace>\<Gamma>\<rbrace>"
+  by (rule parallel_HSem_ind_different_ESem[OF pointwise_adm[OF similar_admI]])
+     (auto simp add: evalHeap_similar)
+
+end
