thys/Launchbury/Env.thy
@@ -1,0 +1,170 @@
+theory Env
+  imports Main HOLCF
+begin
+
+default_sort type
+
+text {*
+Our type for environments is a function with a pcpo as the co-domain; this theory collects
+related definitions.
+*}
+
+subsubsection {* The domain of a pcpo-valued function *}
+
+definition edom :: "('key \<Rightarrow> 'value::pcpo) \<Rightarrow> 'key set" where "edom m = {x. m x \<noteq> \<bottom>}"
+
+lemma bot_edom[simp]: "edom \<bottom> = {}" by (simp add: edom_def)
+
+lemma bot_edom2[simp]: "edom (\<lambda>_ . \<bottom>) = {}" by (simp add: edom_def)
+
+lemma edomIff: "(a \<in> edom m) = (m a \<noteq> \<bottom>)" by (simp add: edom_def)
+
+lemma lookup_not_edom: "x \<notin> edom m \<Longrightarrow> m x = \<bottom>"  by (auto iff:edomIff)
+
+lemma lookup_edom[simp]: "m x \<noteq> \<bottom> \<Longrightarrow> x \<in> edom m"  by (auto iff:edomIff)
+
+subsubsection {* Updates *}
+
+lemma edom_fun_upd_subset: "edom (h (x := v)) \<subseteq> insert x (edom h)"
+  by (auto simp add: edom_def)
+
+declare fun_upd_same[simp] fun_upd_other[simp]
+
+subsubsection {* Restriction *}
+
+definition env_restr :: "'a set \<Rightarrow> ('a \<Rightarrow> 'b::pcpo) \<Rightarrow> ('a \<Rightarrow> 'b)"
+  where "env_restr S m = (\<lambda> x. if x \<in> S then m x else \<bottom>)"
+
+abbreviation env_restr_rev  (infixl "f|`"  110) where "env_restr_rev m S \<equiv> env_restr S m"
+
+notation (latex output) env_restr_rev ("_|\<^bsub>_\<^esub>")
+
+lemma env_restr_empty[simp]: "edom m \<inter> S = {} \<Longrightarrow> m f|` S = \<bottom>"
+  by (fastforce simp add: edom_def env_restr_def)
+
+lemma lookup_env_restr[simp]: "x \<in> S \<Longrightarrow> (env_restr S m) x = m x"
+  by (fastforce simp add: env_restr_def)
+
+lemma lookup_env_restr_not_there[simp]: "x \<notin> S \<Longrightarrow> (env_restr S m) x = \<bottom>"
+  by (fastforce simp add: env_restr_def)
+
+lemma lookup_env_restr_eq: "(m f|` S) x = (if x \<in> S then m x else \<bottom>)"
+  by simp
+
+lemma env_restr_eqI: "(\<And>x. x \<in> S \<Longrightarrow> m\<^sub>1 x = m\<^sub>2 x) \<Longrightarrow> m\<^sub>1 f|` S = m\<^sub>2 f|` S"
+  by (auto simp add: lookup_env_restr_eq)
+
+lemma env_restr_env_restr[simp]:
+ "x f|` d2 f|` d1 = x f|` (d1 \<inter> d2)"
+  by (fastforce simp add: env_restr_def)
+
+lemma env_restr_env_restr_subset:
+ "d1 \<subseteq> d2 \<Longrightarrow> x f|` d2 f|` d1 = x f|` d1"
+ by (metis Int_absorb2 env_restr_env_restr)
+
+lemma env_restr_useless: "edom m \<subseteq> S \<Longrightarrow> m f|` S = m"
+  by (rule ext) (auto simp add: lookup_env_restr_eq dest!: set_mp)
+
+lemma env_restr_UNIV[simp]: "m f|` UNIV = m"
+  by (rule env_restr_useless) simp
+
+lemma env_restr_fun_upd[simp]: "x \<in> S \<Longrightarrow> m1(x := v) f|` S = (m1 f|` S)(x := v)"
+  apply (rule ext)
+  apply (case_tac "xa = x")
+  apply (auto simp add: lookup_env_restr_eq)
+  done
+
+lemma env_restr_fun_upd_other[simp]: "x \<notin> S \<Longrightarrow> m1(x := v) f|` S = m1 f|` S"
+  apply (rule ext)
+  apply (case_tac "xa = x")
+  apply (auto simp add: lookup_env_restr_eq)
+  done
+
+lemma env_restr_eq_subset:
+  assumes "S \<subseteq> S'"
+  and "m1 f|` S' = m2 f|` S'"
+  shows "m1 f|` S = m2 f|` S"
+using assms
+by (metis env_restr_env_restr le_iff_inf)
+
+subsubsection {* Deleting *}
+
+definition env_delete :: "'a \<Rightarrow> ('a \<Rightarrow> 'b) \<Rightarrow> ('a \<Rightarrow> 'b::pcpo)"
+  where "env_delete x m = m(x := \<bottom>)"
+
+lemma lookup_env_delete[simp]:
+  "x' \<noteq> x \<Longrightarrow> env_delete x m x' = m x'"
+  by (simp add: env_delete_def)
+
+lemma lookup_env_delete_None[simp]:
+  "env_delete x m x = \<bottom>"
+  by (simp add: env_delete_def)
+
+lemma edom_env_delete[simp]:
+  "edom (env_delete x m) = edom m - {x}"
+  by (auto simp add: env_delete_def edom_def)
+
+lemma edom_env_delete_subset:
+  "edom (env_delete x m) \<subseteq> edom m" by auto
+
+lemma env_delete_fun_upd[simp]:
+  "env_delete x (m(x := v)) = env_delete x m"
+  by (auto simp add: env_delete_def)
+
+lemma env_delete_fun_upd2[simp]:
+  "(env_delete x m)(x := v) = m(x := v)"
+  by (auto simp add: env_delete_def)
+
+lemma env_delete_fun_upd3[simp]:
+  "x \<noteq> y \<Longrightarrow> env_delete x (m(y := v)) = (env_delete x m)(y := v)"
+  by (auto simp add: env_delete_def)
+
+lemma env_delete_noop[simp]:
+  "x \<notin> edom m \<Longrightarrow> env_delete x m = m"
+  by (auto simp add: env_delete_def edom_def)
+
+lemma fun_upd_env_delete[simp]: "x \<in> edom \<Gamma> \<Longrightarrow> (env_delete x \<Gamma>)(x := \<Gamma> x) = \<Gamma>"
+  by (auto)
+
+lemma env_restr_env_delete_other[simp]: "x \<notin> S \<Longrightarrow> env_delete x m f|` S = m f|` S"
+  apply (rule ext)
+  apply (auto simp add: lookup_env_restr_eq)
+  by (metis lookup_env_delete)
+
+lemma env_delete_restr: "env_delete x m = m f|` (-{x})"
+  by (auto simp add: lookup_env_restr_eq)
+
+subsubsection {* Merging of two functions *}
+
+text {*
+We'd like to have some nice syntax for @{term "override_on"}.
+*}
+
+abbreviation override_on_syn ("_ ++\<^bsub>_\<^esub> _" [100, 0, 100] 100) where "f1 ++\<^bsub>S\<^esub> f2 \<equiv> override_on f1 f2 S"
+
+lemma override_on_bot[simp]:
+  "\<bottom> ++\<^bsub>S\<^esub> m = m f|` S" 
+  "m ++\<^bsub>S\<^esub> \<bottom> = m f|` (-S)" 
+  by (auto simp add: override_on_def env_restr_def)
+
+lemma edom_override_on[simp]: "edom (m1 ++\<^bsub>S\<^esub> m2) = (edom m1 - S) \<union> (edom m2 \<inter> S)"
+  by (auto simp add: override_on_def edom_def)
+
+lemma lookup_override_on_eq: "(m1 ++\<^bsub>S\<^esub> m2) x = (if x \<in> S then m2 x else m1 x)"
+  by (cases "x \<notin> S") simp_all
+
+lemma override_on_upd_swap: 
+  "x \<notin> S \<Longrightarrow> \<rho>(x := z) ++\<^bsub>S\<^esub> \<rho>' = (\<rho> ++\<^bsub>S\<^esub> \<rho>')(x := z)"
+  by (auto simp add: override_on_def  edom_def)
+
+lemma override_on_upd: 
+  "x \<in> S \<Longrightarrow> \<rho> ++\<^bsub>S\<^esub> (\<rho>'(x := z)) = (\<rho> ++\<^bsub>S - {x}\<^esub> \<rho>')(x := z)"
+  by (auto simp add: override_on_def  edom_def)
+
+lemma env_restr_add: "(m1 ++\<^bsub>S2\<^esub> m2) f|` S = m1 f|` S ++\<^bsub>S2\<^esub> m2 f|` S"
+  by (auto simp add: override_on_def  edom_def env_restr_def)
+
+lemma env_delete_add: "env_delete x (m1 ++\<^bsub>S\<^esub> m2) = env_delete x m1 ++\<^bsub>S - {x}\<^esub> env_delete x m2"
+  by (auto simp add: override_on_def  edom_def env_restr_def env_delete_def)
+
+end
