thys/Launchbury/Substitution.thy
@@ -1,0 +1,242 @@
+theory Substitution
+imports Terms
+begin
+
+text {* Defining a substitution function on terms turned out to be slightly tricky. *}
+
+fun subst_var :: "var \<Rightarrow> var \<Rightarrow> var \<Rightarrow> var" ("_[_::v=_]" [1000,100,100] 1000)
+  where "x[y ::v= z] = (if x = y then z else x)"
+
+(* Helper lemmas provided by Christian Urban *)
+
+lemma Projl_permute:
+  assumes a: "\<exists>y. f = Inl y"
+  shows "(p \<bullet> (Sum_Type.Projl f)) = Sum_Type.Projl (p \<bullet> f)"
+using a by auto
+
+lemma Projr_permute:
+  assumes a: "\<exists>y. f = Inr y"
+  shows "(p \<bullet> (Sum_Type.Projr f)) = Sum_Type.Projr (p \<bullet> f)"
+using a by auto
+
+nominal_primrec  (default "sum_case (\<lambda>x. Inl undefined) (\<lambda>x. Inr undefined)",
+                  invariant "\<lambda> a r . (\<forall> as y z . ((a = Inr (as, y, z) \<and> atom ` domA as \<sharp>* (y, z)) \<longrightarrow> map (\<lambda>x . atom (fst x))  (Sum_Type.Projr r) = map (\<lambda>x . atom (fst x)) as))")
+  subst :: "exp \<Rightarrow> var \<Rightarrow> var \<Rightarrow> exp" ("_[_::=_]" [1000,100,100] 1000)
+and
+  subst_heap :: "heap \<Rightarrow> var \<Rightarrow> var \<Rightarrow> heap" ("_[_::h=_]" [1000,100,100] 1000)
+where
+  "(Var x)[y ::= z] = Var (x[y ::v= z])"
+ |"(App e v)[y ::= z] = App (e[y ::= z]) (v[y ::v= z])"
+ |"atom ` domA as \<sharp>* (y,z) \<Longrightarrow> (Let as body)[y ::= z] = Let (as[y ::h= z]) (body[y ::= z])" 
+ |"atom x \<sharp> (y,z) \<Longrightarrow> (Lam [x].e)[y ::= z] = Lam [x].(e[y::=z])"
+ |"[][y ::h= z] = []"
+ |"((v,e)# as)[y ::h= z] = (v, e[y ::= z])# (as[y ::h= z])"
+proof-
+
+have eqvt_at_subst: "\<And> e y z . eqvt_at subst_subst_heap_sumC (Inl (e, y, z)) \<Longrightarrow> eqvt_at (\<lambda>(a, b, c). subst a b c) (e, y, z)"
+  apply(simp add: eqvt_at_def subst_def)
+  apply(rule)
+  apply(subst Projl_permute)
+  apply(thin_tac "?X")+
+  apply (simp add: subst_subst_heap_sumC_def)
+  apply (simp add: THE_default_def)
+  apply (case_tac "Ex1 (subst_subst_heap_graph (Inl (e, y, z)))")
+  apply(simp)
+  apply(auto)[1]
+  apply (erule_tac x="x" in allE)
+  apply simp
+  apply(cases rule: subst_subst_heap_graph.cases)
+  apply(assumption)
+  apply(rule_tac x="Sum_Type.Projl x" in exI)
+  apply(clarify)
+  apply (rule the1_equality)
+  apply blast 
+  apply(simp (no_asm) only: Projl.simps)
+  apply(rule_tac x="Sum_Type.Projl x" in exI)
+  apply(clarify)
+  apply (rule the1_equality)
+  apply blast 
+  apply(simp (no_asm) only: Projl.simps)
+  apply(rule_tac x="Sum_Type.Projl x" in exI)
+  apply(clarify)
+  apply (rule the1_equality)
+  apply blast 
+  apply(simp (no_asm) only: Projl.simps)
+  apply(rule_tac x="Sum_Type.Projl x" in exI)
+  apply(clarify)
+  apply (rule the1_equality)
+  apply blast 
+  apply(simp (no_asm) only: Projl.simps)
+  apply (metis Inr_not_Inl)
+  apply (metis Inr_not_Inl)
+  apply(simp)
+  apply(perm_simp)
+  apply(simp)
+done
+
+have eqvt_at_subst_heap: "\<And> as y z . eqvt_at subst_subst_heap_sumC (Inr (as, y, z)) \<Longrightarrow> eqvt_at (\<lambda>(a, b, c). subst_heap a b c) (as, y, z)"
+  apply(simp add: eqvt_at_def subst_heap_def)
+  apply(rule)
+  apply(subst Projr_permute)
+  apply(thin_tac "?X")+
+  apply (simp add: subst_subst_heap_sumC_def)
+  apply (simp add: THE_default_def)
+  apply (case_tac "Ex1 (subst_subst_heap_graph (Inr (as, y, z)))")
+  apply(simp)
+  apply(auto)[1]
+  apply (erule_tac x="x" in allE)
+  apply simp
+  apply(cases rule: subst_subst_heap_graph.cases)
+  apply(assumption)
+  apply (metis (mono_tags) Inr_not_Inl)+
+  apply(rule_tac x="Sum_Type.Projr x" in exI)
+  apply(clarify)
+  apply (rule the1_equality)
+  apply auto[1]
+  apply(simp (no_asm) only: Projr.simps)
+  
+  apply(rule_tac x="Sum_Type.Projr x" in exI)
+  apply(clarify)
+  apply (rule the1_equality)
+  apply auto[1]
+  apply(simp (no_asm) only: Projr.simps)
+  
+  apply(simp)
+  apply(perm_simp)
+  apply(simp)
+done
+
+{
+(* Equivariance of the graph *)
+case goal1 thus ?case
+  unfolding eqvt_def subst_subst_heap_graph_aux_def
+  by simp
+
+(* The invariant *)
+next case goal2 thus ?case
+  by (induct rule: subst_subst_heap_graph.induct)(auto simp add: exp_assn.bn_defs fresh_star_insert)
+
+(* Exhaustiveness *)
+next case (goal3 P x) show ?case
+  proof(cases x)
+  case (Inl a) thus P
+    proof(cases a)
+    case (fields a1 a2 a3)
+    thus P using Inl goal3
+      apply (rule_tac y ="a1" and c ="(a2, a3)" in exp_strong_exhaust)
+      apply (auto simp add: fresh_star_def)
+      apply metis
+    done
+  qed
+  next
+  case (Inr a) thus P
+    proof (cases a)
+    case (fields a1 a2 a3)
+    thus P using Inr goal3
+      by (metis heapToAssn.cases)
+  qed
+qed
+
+next case (goal15 e y2 z2 as e2 y z as2) thus ?case
+  apply -
+  apply (drule eqvt_at_subst)+
+  apply (drule eqvt_at_subst_heap)+
+  apply (simp only: meta_eq_to_obj_eq[OF subst_def, symmetric, unfolded fun_eq_iff]
+    meta_eq_to_obj_eq[OF subst_heap_def, symmetric, unfolded fun_eq_iff])
+  (* No _sum any more at this point! *)
+  apply (auto simp add: Abs_fresh_iff)
+  apply (drule_tac
+    c = "(y, z)" and
+    as = "(map (\<lambda>x. atom (fst x)) e)" and
+    bs = "(map (\<lambda>x. atom (fst x)) e2)" and
+    f = "\<lambda> a b c . [a]lst. (subst (fst b) y z, subst_heap (snd b) y z )" in Abs_lst_fcb2)
+  apply (simp add: perm_supp_eq fresh_Pair fresh_star_def Abs_fresh_iff)
+  apply (metis domA_def image_image image_set)
+  apply (metis domA_def image_image image_set)
+  apply (simp add: eqvt_at_def, simp add: fresh_star_Pair perm_supp_eq)
+  apply (simp add: eqvt_at_def, simp add: fresh_star_Pair perm_supp_eq)
+  apply (simp add: eqvt_at_def)
+  done
+
+next case (goal19 x2 y2 z2 e2 x y z e) thus ?case
+  apply -
+  apply (drule eqvt_at_subst)+
+  apply (simp only: Abs_fresh_iff meta_eq_to_obj_eq[OF subst_def, symmetric, unfolded fun_eq_iff])
+  (* No _sum any more at this point! *)
+  apply (simp add: eqvt_at_def)
+  apply rule
+  apply (erule_tac x = "(x2 \<leftrightarrow> c)" in allE)
+  apply (erule_tac x = "(x \<leftrightarrow> c)" in allE)
+  apply auto
+  done
+}
+qed(auto)
+
+termination (eqvt) by lexicographic_order
+
+lemma shows
+  True and bn_subst[simp]: "domA (subst_heap as y z) = domA as"
+by(induct rule:subst_subst_heap.induct)
+  (auto simp add: exp_assn.bn_defs fresh_star_insert)
+
+lemma subst_noop[simp]:
+shows "e[y ::= y] = e" and "as[y::h=y]= as"
+by(induct e y y and as y y rule:subst_subst_heap.induct)
+  (auto simp add:fresh_star_Pair exp_assn.bn_defs)
+
+lemma subst_is_fresh[simp]:
+assumes "atom y \<sharp> z"
+shows
+  "atom y \<sharp> e[y ::= z]"
+and
+ "atom ` domA as \<sharp>* y \<Longrightarrow> atom y \<sharp> as[y::h=z]"
+using assms
+by(induct e y z and as y z rule:subst_subst_heap.induct)
+  (auto simp add:fresh_at_base fresh_star_Pair fresh_star_insert fresh_Nil fresh_Cons)
+
+lemma
+ subst_pres_fresh: "x \<sharp> e \<Longrightarrow> x \<sharp> z \<Longrightarrow> x \<sharp> e[y ::= z]"
+and
+ "x \<sharp> \<Gamma> \<Longrightarrow> x \<sharp> z \<Longrightarrow> x \<notin> atom ` domA \<Gamma> \<Longrightarrow> x \<sharp> (\<Gamma>[y ::h= z])"
+by(induct e y z and \<Gamma> y z rule:subst_subst_heap.induct)
+  (auto simp add:fresh_star_Pair exp_assn.bn_defs fresh_Cons)
+
+lemma subst_fresh_noop: "atom x \<sharp> e \<Longrightarrow> e[x ::= y] = e"
+  and subst_heap_fresh_noop: "atom x \<sharp> \<Gamma> \<Longrightarrow>  \<Gamma>[x ::h= y] = \<Gamma>"
+by (nominal_induct  e and \<Gamma> avoiding: x y rule:exp_heap_strong_induct)
+  (auto simp add: fresh_star_def fresh_Pair fresh_at_base fresh_Cons simp del: exp_assn.eq_iff)
+
+lemma supp_subst: "supp (e[y::=x]) \<subseteq> (supp e - {atom y}) \<union> supp x"
+proof-
+  have "\<And> a. (a \<sharp> e \<or> a = atom y) \<Longrightarrow> a \<sharp> x \<Longrightarrow> a \<sharp> e[y::=x]"
+    by (auto intro: subst_pres_fresh)
+  thus ?thesis by (auto simp add: fresh_def)
+qed
+
+lemma fv_subst_subset: "fv (e[y ::= x]) \<subseteq> (fv e - {y}) \<union> {x}"
+proof-
+  have "fv (e[y ::= x]) = {v. atom v \<in> supp (e[y ::= x])}" unfolding fv_def..
+  also have "\<dots> \<subseteq> {v. atom v \<in> ((supp e - {atom y}) \<union> supp x)}"
+    using supp_subst by auto
+  also have "\<dots> = (fv e - {y}) \<union> {x}"
+    using supp_subst by (auto simp add: fv_def supp_at_base)
+  finally show ?thesis.
+qed
+
+lemma fresh_star_at_base:
+  fixes x :: "'a :: at_base"
+  shows "S \<sharp>* x \<longleftrightarrow> atom x \<notin> S"
+  by (metis fresh_at_base(2) fresh_star_def)
+
+lemma subst_swap_same: "atom x \<sharp> e \<Longrightarrow>  (x \<leftrightarrow> y) \<bullet> e = e[y ::=x]"
+  and "atom x \<sharp> \<Gamma> \<Longrightarrow> atom `domA \<Gamma> \<sharp>* y \<Longrightarrow> (x \<leftrightarrow> y) \<bullet> \<Gamma> = \<Gamma>[y ::h= x]"
+by(nominal_induct  e and \<Gamma> avoiding: x y rule:exp_heap_strong_induct)
+  (auto simp add: fresh_star_Pair fresh_star_at_base fresh_Cons simp del: exp_assn.eq_iff)
+
+lemma subst_subst_back: "atom x \<sharp> e \<Longrightarrow>  e[y::=x][x::=y] = e" 
+  and "atom x \<sharp> \<Gamma> \<Longrightarrow> atom `domA \<Gamma> \<sharp>* y  \<Longrightarrow> \<Gamma>[y::h=x][x::h=y] = \<Gamma>"
+by(nominal_induct  e and \<Gamma> avoiding: x y rule:exp_heap_strong_induct)
+  (auto simp add: fresh_star_Pair fresh_star_at_base fresh_star_Cons fresh_Cons  exp_assn.bn_defs simp del: exp_assn.eq_iff)
+
+
+end
