thys/Launchbury/Value.thy
@@ -1,0 +1,54 @@
+theory "Value"
+  imports HOLCF
+begin
+
+subsubsection {* The semantic domain for values and environments *}
+
+domain Value = Fn (lazy "Value \<rightarrow> Value")
+
+fixrec Fn_project :: "Value \<rightarrow> Value \<rightarrow> Value"
+ where "Fn_project\<cdot>(Fn\<cdot>f) = f"
+
+abbreviation Fn_project_abbr (infix "\<down>Fn" 55)
+  where "f \<down>Fn v \<equiv> Fn_project\<cdot>f\<cdot>v"
+
+lemma [simp]: "\<bottom> \<down>Fn x = \<bottom>"
+  by (fixrec_simp)
+
+text {*
+A chain in the domain @{typ Value} is either always bottom, or eventually @{term "Fn"} of another
+chain
+*}
+
+lemma Value_chainE:
+  assumes "chain Y"
+  obtains "Y = (\<lambda> _ . \<bottom>)" |
+          n Y' where "Y = (\<lambda> m. (if m < n then \<bottom> else Fn\<cdot>(Y' (m-n))))" "chain Y'"
+proof(cases "Y = (\<lambda> _ . \<bottom>)")
+  case True
+  thus ?thesis by (rule that(1))
+next
+  case False
+  hence "\<exists> i. Y i \<noteq> \<bottom>" by auto
+  hence "\<exists> n. Y n \<noteq> \<bottom> \<and> (\<forall>m. Y m \<noteq> \<bottom> \<longrightarrow> m \<ge> n)"
+    by (rule exE)(rule ex_has_least_nat)
+  then obtain n where "Y n \<noteq> \<bottom>" and "\<forall>m. m < n \<longrightarrow> Y m = \<bottom>" by fastforce
+  then obtain f where "Y n = Fn \<cdot> f" by (metis Value.exhaust)
+  {
+    fix i
+    from `chain Y` have "Y n \<sqsubseteq> Y (i+n)" by (metis chain_mono le_add2)  
+    with `Y n = _`
+    have "\<exists> g. (Y (i+n) = Fn \<cdot> g)" by (metis (full_types) Value.exhaust minimal po_eq_conv)
+  }
+  then obtain Y' where Y': "\<And> i. Y (i + n) = Fn \<cdot> (Y' i)" by metis 
+
+  have "Y = (\<lambda>m. if m < n then \<bottom> else Fn\<cdot>(Y' (m - n)))"
+      using `\<forall>m. _` Y' by (metis add_diff_inverse nat_add_commute)
+  moreover
+  have"chain Y'" using `chain Y`
+    by (auto intro!:chainI elim: chainE  simp add: Value.inverts[symmetric] Y'[symmetric] simp del: Value.inverts)
+  ultimately
+  show ?thesis by (rule that(2))
+qed
+
+end
